---
layout: post
title: 测试公式
date: 2019-07-24
Author: 来自中世界
categories: 
tags: [sample, document]
comments: true
---

$$
\begin{align*}
y = y(x,t) &= A e^{i\theta} \\
&= A (\cos \theta + i \sin \theta) \\
&= A (\cos(kx - \omega t) + i \sin(kx - \omega t)) \\
&= A\cos(kx - \omega t) + i A\sin(kx - \omega t)  \\
&= A\cos \Big(\frac{2\pi}{\lambda}x - \frac{2\pi v}{\lambda} t \Big) + i A\sin \Big(\frac{2\pi}{\lambda}x - \frac{2\pi v}{\lambda} t \Big)  \\
&= A\cos \frac{2\pi}{\lambda} (x - v t) + i A\sin \frac{2\pi}{\lambda} (x - v t)
\end{align*}
$$


$\ce{CH4 + 2 $\left( \ce{O2 + 79/21 N2} \right)$}$


$$
x+1\over\sqrt{1-x^2}\label{ref1}
$$